beluga_clean/meta.v
@@ -1,4 +1,6 @@
 Require Export util.
+Require Import Coq.Logic.FunctionalExtensionality.
+Require Import Setoid.
 Set Implicit Arguments.
 
 Axiom mtype : world -> Set.
@@ -18,6 +20,9 @@ Axiom app_msubst_assoc : forall {δ} (t:meta_term δ)
  {δ'} (θ:msubst δ δ') {δ''} (θ':msubst δ' δ''),
  app_msubst θ' (app_msubst θ t) =
  app_msubst (app_msubst θ' ○ θ) t.
+Axiom app_msubst_mvar : forall {δ δ'} (θ:msubst δ δ')
+  (n:name δ), app_msubst θ (m_var n) = θ n.
+Axiom mvar_unit : forall δ, app_msubst (@m_var δ) = id.
 
 Class substitutable (A:world -> Set) := {
    app_subst : forall {α β}, msubst α β -> A α -> A β ;
@@ -40,9 +45,128 @@ Instance mtype_substitutable : substitutable mtype := {
   assoc := @app_msubst_mtype_assoc
  }.
 
-Definition single_subst {γ γ'} (x:γ↪γ') {T} `{H:substitutable T} (N:meta_term γ) (M:T γ') :=
- 〚@m_var γ,,(x,N)〛 M.
+Definition single_subst {γ γ'} (x:γ↪γ') (N:meta_term γ) : msubst γ' γ :=
+ (@m_var γ,,(x,N)).
 
 (* TODO: This may cause me trouble later *)
 Definition msubst_oft {α} (Δ:mtype_assign α) {β} (Δ':mtype_assign β) θ := forall x, Δ' ⊨ (θ x) ∷ 〚θ〛(Δ x).
 Notation "Δ' ⊩ θ ∷ Δ" := (@msubst_oft _ Δ _ Δ' θ) (at level 90).
+
+Ltac clean_msubsts :=
+(match goal with
+ | [ H : _ |- context f [app_msubst ?t ?T]] =>
+   replace (app_msubst t T) with (〚 t 〛 T);
+   try reflexivity
+ | _ => fail
+end).
+
+Definition context_mult {δ δ'} (θ:msubst δ δ') {δ'' δ'''} (y:δ'↪δ''') (x:δ↪δ'') := (〚@m_var _ ○ ↑y〛 ○ θ,, (x,y)).
+Notation "θ × ( y // x )" := (context_mult θ y x) (at level 10).
+
+Lemma compose_cons :
+  forall δ δ' β γ
+  (s : δ ↪ δ')
+  (θ : msubst δ β) (θ' : msubst β γ) C,
+  (〚θ'〛 ○ (θ,, (s,C))) =
+   ((〚θ'〛 ○ θ),, (s,〚θ'〛C)).
+intros. eapply functional_extensionality. intros.
+unfold compose at 1 2 3.
+destruct (export s x); reflexivity.
+Qed.
+
+Lemma compose_mvar {α β} (θ:msubst α β) : 〚θ〛○(@m_var _) = θ.
+apply functional_extensionality.
+apply app_msubst_mvar.
+Qed.
+
+Lemma subst_assoc {α β γ δ} (θ1:msubst α β) θ2 (θ3:msubst γ δ) :
+ 〚〚θ3〛 ○ θ2〛 ○ θ1 = 〚θ3〛 ○ (〚θ2〛 ○ θ1).
+apply functional_extensionality. intros.
+unfold compose at 1 3 4.
+erewrite assoc.
+reflexivity.
+Qed.
+
+Lemma cons_import {α β γ} (θ:msubst α β) (x:α↪γ) C :
+ (θ,,(x,C)) ○ (↑x) = θ.
+apply functional_extensionality. intro.
+unfold compose.
+erewrite export_import_inv.
+reflexivity.
+Qed.
+
+Lemma cons_self {α β γ} (θ:msubst α β) (x:α↪γ) C :
+ (〚θ,,(x,C)〛 (m_var x)) = C.
+erewrite app_msubst_mvar.
+unfold compose. erewrite export_self. reflexivity.
+Qed.
+
+Lemma assoc' {α β γ} {T} `{H:substitutable T} (θ1:msubst α β)
+(θ2:msubst β γ) :
+ 〚〚θ2〛 ○ θ1〛 = 〚θ2〛 ○ 〚θ1〛.
+apply functional_extensionality. intro.
+unfold compose.
+erewrite assoc.
+reflexivity.
+Qed.
+
+Lemma compose_product :
+  forall δ δ' β γ x x0
+  (s : δ ↪ δ')
+  (θ : msubst δ β) (θ' : msubst β γ) 
+  (s0 : γ ↪ x) (s1 : β ↪ x0),
+  (〚(θ' ×  (s0 // s1))〛 ○ (θ ×  (s1 // s))) =
+   (〚θ'〛 ○ θ) ×  (s0 // s).
+intros.
+unfold context_mult.
+erewrite compose_cons.
+erewrite cons_self.
+f_equal.
+f_equal.
+erewrite <- subst_assoc.
+erewrite compose_assoc.
+erewrite compose_assoc.
+f_equal.
+erewrite compose_mvar.
+erewrite cons_import.
+apply assoc'.
+Qed.
+
+Lemma single_subst_mult {α α' β β'} (θ:msubst α β)
+(z:β↪β') (y:α↪α') C :
+ 〚single_subst z C〛 ○ (θ × (z // y)) = (θ,, (y,C)).
+unfold single_subst.
+unfold context_mult.
+erewrite compose_cons.
+erewrite cons_self.
+erewrite compose_assoc.
+erewrite <- assoc'.
+erewrite compose_assoc.
+erewrite compose_mvar.
+erewrite cons_import.
+erewrite mvar_unit.
+erewrite id_unit_left.
+reflexivity.
+Qed.
+
+Lemma msubst_over_single {α β γ} (θ:msubst α β) (x:α↪γ) C :
+ 〚θ〛 ○ (single_subst x C) = (θ,, (x,〚θ〛C)). 
+unfold single_subst.
+erewrite compose_cons.
+erewrite compose_mvar.
+reflexivity.
+Qed.
+
+Lemma common_var {α α' β β' γ γ'} {θ:msubst α β} {θ':msubst γ β}
+                 {x:α↪α'} {y:γ↪γ'} {z:β↪β'} {T}
+                 `{H:substitutable T} {M:T γ'} {N:T α'} C :
+   〚θ' × (z // y)〛 M = 〚θ × (z // x)〛 N
+-> 〚θ',, (y,C)〛    M = 〚θ,, (x,C)〛    N.
+intro.
+assert (〚single_subst z C〛 (〚θ' × (z // y) 〛 M)
+     = (〚single_subst z C〛 (〚θ  × (z // x) 〛 N)))
+ by (f_equal; auto).
+erewrite assoc in H1. erewrite single_subst_mult in H1.
+erewrite assoc in H1. erewrite single_subst_mult in H1.
+assumption.
+Qed.
