beluga_clean/util.v
@@ -1,13 +1,43 @@
 Require Export worlds.
+Require Import Coq.Logic.FunctionalExtensionality.
 
- Definition cdot {A} : name ∅ -> A := fun n => match (empty_is_empty n) with end.
- Notation "·" := cdot.
+Definition cdot {A} : name ∅ -> A := fun n => match (empty_is_empty n) with end.
+Notation "·" := cdot.
 
- Definition maybe {A C} (f:A -> C) (c:C) (x:A + unit) : C := match x with | inl a => f a | inr _ => c end.  
+Definition maybe {A C} (f:A -> C) (c:C) (x:A + unit) : C := match x with | inl a => f a | inr _ => c end.  
 
 Definition compose {A B C:Set} (f:A -> B) (g:B -> C) (a:A) : C
  := g (f a). 
 
 Notation "f ○ g" := (compose g f) (at level 10).
 
+Definition id {A:Set} := fun x:A => x.
+
 Notation "Γ ,, ( y , t )" := ((maybe Γ t) ○ (export y)) (at level 90).
+
+Lemma compose_assoc {A B C D:Set} (f:A -> B) g (h:C -> D) :
+ h ○ (g ○ f) = (h ○ g) ○ f.
+apply functional_extensionality.
+unfold compose. reflexivity.
+Qed.
+
+Lemma compose_def {A B C:Set} (f:A->B) (g:B -> C) :
+ g ○ f = fun x => g (f x).
+reflexivity.
+Qed.
+Lemma compose_def' {A B C:Set} (f:A->B) (g:B -> C) x :
+ g (f x) = (g ○ f) x.
+reflexivity.
+Qed.
+
+Lemma id_unit_left {A B:Set} (f:A -> B) : id ○ f = f.
+apply functional_extensionality. unfold compose. reflexivity.
+Qed.
+
+Lemma id_unit_right {A B:Set} (f:A -> B) : f ○ id = f.
+apply functional_extensionality. unfold compose. reflexivity.
+Qed.
+
+Lemma eta {A B:Set} (f:A -> B) : (fun x => f x) = f.
+apply functional_extensionality. reflexivity.
+Qed.
