beluga_clean/worlds.v
@@ -8,11 +8,12 @@ Notation "α ↪ β" := (link α β) (at level 90).
 
 Parameter toName : forall {α β}, α↪β -> name β.
 Coercion toName : link >-> name.
-Axiom import : forall {α β}, α↪β -> name α -> name β.
+Definition name_subst α β := name α -> name β.
+Axiom import : forall {α β}, α↪β -> name_subst α β.
 Notation "↑ x" := (import x) (at level 90).
 Parameter succ_world : world -> world.
 Parameter succ_link : forall α, α↪(succ_world α).
-
+Notation "₁" := (succ_link ∅).
 Axiom export : forall {α β} (y:α↪β) (n:name β), name α + unit.
 Axiom export_self : forall {α β} (y:α↪β), export y y = inr _ tt.
 Axiom export_import_inv : forall {α β} (y:α↪β) (n:name α), export y (import y n) = inl _ n.
